use deep embeddings for constrained monads, add some explanations.

ParserCombinators/Memoized.lean
@@ -14,7 +14,7 @@ import Aesop
 
 -- β is the alphabet: parsers work over Array β
 universe u v
-variable {τ} { α β : Type u } {tag : τ → Type u} { μ : Type u → Type u } [BEq β] [BEq τ] [LawfulBEq τ] [Hashable τ] [DecidableEq τ] [SemilatticeAlt μ] [∀ t : τ, DecidableEq (tag t)]
+variable {τ} { α β : Type u } {tag : τ → Type u} { μ : Type u → Type u } [BEq β] [BEq τ] [LawfulBEq τ] [Hashable τ] [DecidableEq τ] [SemilatticeAlt μ] [h_eq : ∀ t : τ, DecidableEq (tag t)]
 
 def startState {μ} [Monad μ] : MemoData tag μ :=
   Std.DHashMap.emptyWithCapacity
@@ -31,8 +31,27 @@ def joinUnderCache {γ} [Max (μ γ)] [Bot (μ γ)] [Monad μ] (s1 s2 : MStateT 
   liftA2 (fun m1 m2 => Std.HashMap.unionSup m1 m2) s1 s2
 
 -- Some of the α's here should become existential/hidden
-abbrev Parser (β : Type u) (μ : Type u → Type u) [Monad μ] [SemilatticeAlt μ] (α : Type u) :=
+abbrev Parser
+  {τ} {tag : τ → Type u} [BEq τ] [LawfulBEq τ] [Hashable τ] [DecidableEq τ] [∀ t : τ, DecidableEq (tag t)]
+  (β : Type u) (μ : Type u → Type u) [Monad μ] [SemilatticeAlt μ] (α : Type u) :=
   ℕ → MStateT (MemoData tag μ) (ReaderM (Array β)) (Std.HashMap ℕ (μ α))
+
+namespace Parser
+variable [Monad μ] [Traversable μ]
+def bind [DecidableEq β'] (x : Parser (tag := tag) β μ α) (f : α → Parser (tag := tag) β μ β')
+  := fun pos => do
+    let pivotToResult ← x pos
+    let actions : List (μ (MStateT (MemoData tag μ) (ReaderM (Array β)) (Std.HashMap ℕ (μ β')))) :=
+      pivotToResult.toList.map (fun (j, ma) => (fun a => f a j) <$> ma)
+    actions.foldl
+      (Traversable.foldl joinUnderCache)
+      (pure Std.HashMap.emptyWithCapacity)
+
+def failure : Parser (tag := tag) β μ α := fun _pos => pure Std.HashMap.emptyWithCapacity
+
+def orElse [DecidableEq α] (r1 r2 : Parser (tag := tag) β μ α) pos :=
+    joinUnderCache (r1 pos) (r2 pos)
+end Parser
 
 instance [Monad μ] : Functor (Parser (tag := tag) β μ) where
   map f x := Functor.map (Std.HashMap.map (fun _ => Functor.map f)) ∘ x
@@ -42,49 +61,54 @@ instance [Monad μ] : Functor (Parser (tag := tag) β μ) where
 instance [Monad μ] : Pure (Parser (tag := tag) β μ) where
   pure a := fun pos => pure {(pos, pure a)}
 
--- might need other type class instances (e.g. to make fold work)
--- also, you may need to define or find a fold operation for Std.HashMap
-instance [Monad μ] [Traversable μ] [∀ α, Max (μ α)] [∀ α, Bot (μ α)] : Bind (Parser (tag := tag) β μ) where
-  bind {_ β'} x f := fun pos => do
-      let pivotToResult ← x pos
-      let actions : List (μ (MStateT (MemoData tag μ) (ReaderM (Array β)) (Std.HashMap ℕ (μ β')))) :=
-        pivotToResult.toList.map (fun (j, ma) => (fun a => f a j) <$> ma)
-      actions.foldl
-        (Traversable.foldl joinUnderCache)
-        (pure Std.HashMap.emptyWithCapacity)
+-- Deep embedding of Monad for parsers.
+--
+-- From Sculthorpe, et al. <https://dl.acm.org/doi/10.1145/2500365.2500602>
+--
+-- We adapt it to force calculating the join as soon as possible.
+inductive ParserM (β : Type u) (μ : Type u → Type u) [Monad μ] [SemilatticeAlt μ] (α : Type u) where
+  | Return (a : α)
+  | Bind (p : Parser (tag := tag) β μ α') (f : α' → ParserM β μ α)
 
-instance [Monad μ] [Traversable μ] [∀ α, Max (μ α)] [∀ α, Bot (μ α)] : Monad (Parser (tag := tag) β μ) where
+namespace ParserM
+variable [Monad μ] [SemilatticeAlt μ]
+def bind [Monad μ] [Traversable μ] : (ParserM (tag := tag) β μ α') → (α' → ParserM (tag := tag) β μ α) → ParserM (tag := tag) β μ α
+  | ParserM.Return a, k => k a
+  | ParserM.Bind p f, k => ParserM.Bind p (fun x => bind (f x) k)
 
-instance [Monad μ] [Traversable μ] [∀ α, Max (μ α)] [∀ α, Bot (μ α)] : Alternative (Parser (tag := tag) β μ) where
-  failure _pos := pure Std.HashMap.emptyWithCapacity
-  orElse r1 r2 pos :=
-    let s1 := r1 pos
-    let s2 := r2 () pos
-    joinUnderCache s1 s2
+instance [Monad μ] [Traversable μ] : Monad (ParserM (tag := tag) β μ) where
+  pure := ParserM.Return
+  bind := ParserM.bind
 
-instance [Monad μ] [Alternative μ] [Traversable μ] [∀ α, Max (μ α)] [∀ α, Bot (μ α)] : LawfulMonad (Parser (tag := tag) β μ) := by {
-  refine LawfulMonad.mk' (Parser β μ) ?_ ?_ ?_ ?_ ?_ ?_ ?_ ?_
-  · sorry
-  · sorry
-  · sorry
-  · sorry  -- use the proofs for the default impl
-  · sorry  -- use the proofs for the default impl
-  · sorry  -- use the proofs for the default impl
-  · sorry  -- use the proofs for the default impl
-  · sorry  -- use the proofs for the default impl
-}
+def lift (p : Parser (tag := tag) β μ α) : ParserM (tag := tag) β μ α := ParserM.Bind p ParserM.Return
 
-instance [Monad μ] [Alternative μ] [Traversable μ] [∀ α, Max (μ α)] [∀ α, Bot (μ α)] : LawfulAlternative (Parser (tag := tag) β μ) where
-  map_failure := sorry
-  failure_seq := sorry
-  orElse_failure := sorry
-  failure_orElse := sorry
-  orElse_assoc := sorry
-  map_orElse := sorry
+instance [Monad μ] [Traversable μ] [DecidableEq α] : Bot (ParserM (tag := tag) β μ α) where
+  bot := lift Parser.failure
 
-def epsilon [Monad μ] : Parser (tag := tag) β μ PUnit := fun pos => pure {(pos, pure $ PUnit.unit)}
+variable [Monad μ] [Traversable μ] [DecidableEq α]
+def lower : ParserM (tag := tag) β μ α →  Parser (tag := tag) β μ α
+  | ParserM.Return x => pure x
+  | ParserM.Bind x k => Parser.bind x (fun x => lower (k x))
 
-def terminal [Monad μ] (s : String) : Parser (tag := tag) UChar μ UString := fun pos => do
+open ParserM in
+instance [Monad μ] [Traversable μ] [DecidableEq α] : Max (ParserM (tag := tag) β μ α) where
+  max
+  | Return x, Return y => ParserM.Bind (Parser.orElse (Pure.pure x) (Pure.pure y)) Return
+  | Return x, ParserM.Bind y k => lift $ Parser.orElse (pure x) (y.bind (lower ∘ k))
+  | ParserM.Bind x k, Return y => lift $ Parser.orElse (x.bind (lower ∘ k)) (pure y)
+  | ParserM.Bind p₁ k₁, ParserM.Bind p₂ k₂ => lift $ Parser.orElse (p₁.bind (lower ∘ k₁)) (p₂.bind (lower ∘ k₂))
+
+end ParserM
+
+-- TODO: prove that the relevant laws hold for the monad instance
+-- TODO: prove that ParserM is a `SemilatticeSup` + `OrderBot`
+-- TODO: prove that the relevant laws hold for lower/lift
+
+open ParserM (lift lower)
+
+def epsilon [Monad μ] : ParserM (tag := tag) β μ PUnit := lift $ fun pos => pure {(pos, pure $ PUnit.unit)}
+
+def terminal [Monad μ] (s : String) : ParserM (tag := tag) UChar μ UString := lift $ fun pos => do
   let input ← read
   if pos >= 0 && (s.data.map ULift.up).toArray.isPrefixOf (input.extract pos) then
     let endPos := pos + s.length
@@ -92,7 +116,7 @@ def terminal [Monad μ] (s : String) : Parser (tag := tag) UChar μ UString := f
   else
     pure Std.HashMap.emptyWithCapacity
 
-def terminal' [Monad μ] (t: β) : Parser (tag := tag) β μ β := fun pos => do
+def terminal' [Monad μ] (t: β) : ParserM (tag := tag) β μ β := lift $ fun pos => do
   let input ← read
   if pos >= 0 && some t == input[pos]? then
     pure {(pos + 1, pure t)}
@@ -101,8 +125,20 @@ def terminal' [Monad μ] (t: β) : Parser (tag := tag) β μ β := fun pos => do
 
 -- TODO(maemre): this is increasing the memoization table, which is a Noetherian lattice.
 -- We need to make a termination argument using that.
-partial def memoize [Monad μ] [Traversable μ] (g : ((t : τ) → Parser (tag := tag) β μ (tag t)) → (t : τ) → Parser (tag := tag) β μ (tag t)) (t : τ) : Parser (tag := tag) β μ (tag t) :=
-  fun pos => do
+--
+-- We need two more ingredients:
+--
+-- 1. Each tag has correct data, e.g. t ∈ memo → memo.get? t ⊆ memoize g pos
+-- 2. There is a counter for each tag and we saturate it in N steps where N = remaining string
+--    length.  This definition is similar to `withFuel`, and it should work on non-cyclic grammars
+--    as seen in Frost and Hafiz <https://dl.acm.org/doi/10.1145/1149982.1149988>.
+--
+-- (1) will ensure that we always produce correct results.
+-- (2) will ensure that we always terminate.  Ideally, we could try for a fixpoint-like approach
+-- where our initial results are empty and we gradually re-run the parser until it saturates?
+-- This might get tricky, though.
+partial def memoize [Monad μ] [Traversable μ] [DecidableEq α] (g : ((t : τ) → ParserM (tag := tag) β μ (tag t)) → (t : τ) → ParserM (tag := tag) β μ (tag t)) (t : τ) : ParserM (tag := tag) β μ (tag t) :=
+  lift $ fun pos => do
     let memo ← get
     -- Check if we have cached results for this tag and position
     match memo.get? t with
@@ -111,7 +147,7 @@ partial def memoize [Monad μ] [Traversable μ] (g : ((t : τ) → Parser (tag :
       | some cachedResult => pure {(pos, cachedResult)}
       | none =>
         -- No cached result for this position, compute and cache
-        let results ← g (memoize g) t pos
+        let results ← lower (g (memoize g) t) pos
         -- Cache the new results
         let newPositionMap := results.fold (fun acc newPos result =>
           acc.insert newPos result) positionMap
@@ -119,7 +155,7 @@ partial def memoize [Monad μ] [Traversable μ] (g : ((t : τ) → Parser (tag :
         pure results
     | none =>
       -- No entry for this tag at all, so we compute it and cache it
-      let results ← g (memoize g) t pos
+      let results ← lower (g (memoize g) t) pos
       -- Create new position map and cache the results
       let newPositionMap := results.fold (fun acc newPos result =>
         acc.insert newPos result) Std.HashMap.emptyWithCapacity
@@ -130,12 +166,12 @@ partial def memoize [Monad μ] [Traversable μ] (g : ((t : τ) → Parser (tag :
 
 -- Will use `Const` as the concrete monad (some is success, ⊥ is failure, ⊤ is ambiguity)
 
-def runParser [Monad μ] (p : Parser (tag := tag) β μ α) (input : Array β) (pos : ℕ := 0) : (Std.HashMap ℕ (μ α)) × MemoData tag μ :=
-  let stateTResult := (p pos).run startState
+def runParser [Monad μ] [Traversable μ] [DecidableEq α] (p : ParserM (tag := tag) β μ α) (input : Array β) (pos : ℕ := 0) : (Std.HashMap ℕ (μ α)) × MemoData tag μ :=
+  let stateTResult := (p.lower pos).run startState
   let readerResult := stateTResult.run input
   readerResult
 
-def runParser' [Monad μ] (p : Parser (tag := tag) UChar μ α) (input : String) (pos : ℕ := 0) : (Std.HashMap ℕ (μ α)) × MemoData tag μ :=
+def runParser' [Monad μ] [Traversable μ] [DecidableEq α] (p : ParserM (tag := tag) UChar μ α) (input : String) (pos : ℕ := 0) : (Std.HashMap ℕ (μ α)) × MemoData tag μ :=
   runParser p (input.toList.map ULift.up).toArray pos
 
 def emptyTag : PUnit → Type := fun _ => PUnit
@@ -145,7 +181,8 @@ instance (t : PUnit) : DecidableEq (emptyTag t) := by
   infer_instance
 
 def runParserO {μ : Type → Type} {α : Type} [Monad μ] [SemilatticeAlt μ]
-  (p : Parser (tag := emptyTag) UChar μ α) (input : String) (pos : ℕ := 0)
+  [Traversable μ] [DecidableEq α]
+  (p : ParserM (tag := emptyTag) UChar μ α) (input : String) (pos : ℕ := 0)
     : (Std.HashMap ℕ (μ α)) × MemoData emptyTag μ :=
   runParser'.{0} p input pos
 
@@ -167,17 +204,17 @@ def runParserO {μ : Type → Type} {α : Type} [Monad μ] [SemilatticeAlt μ]
 -- Testing instances:
 
 -- Functor (`<$>`)
-def funcParser : Parser (tag := emptyTag) UChar Const String := (fun _ => "matched!") <$> terminal "hello"
-def funcParser2 : Parser (tag := emptyTag) UChar Const ℕ := (fun x => x * 3) <$> terminal "hello" $> 2
+def funcParser : ParserM (tag := emptyTag) UChar Const String := (fun _ => "matched!") <$> terminal "hello"
+def funcParser2 : ParserM (tag := emptyTag) UChar Const ℕ := (fun x => x * 3) <$> terminal "hello" $> 2
 
 -- TODO: (Madi) Just beef this up by testing edge cases
 #guard (runParserO (μ := Const) funcParser "hello world").1.toList == [(5, Const.some "matched!")]
 #guard (runParserO (μ := Const) funcParser "hell").1.toList == []
 #guard (runParserO (μ := Const) funcParser2 "hello").1.toList == [(5, Const.some 6)]
 
--- Alternative (`<|>`)
-def altParser [Monad μ] [Traversable μ] [∀ α, Max (μ α)] [∀ α, Bot (μ α)] : Parser (tag := tag) UChar μ UString :=
-  terminal "hello" <|> terminal "goodbye"
+-- Alternative (`⊔`)
+def altParser [Monad μ] [Traversable μ] : ParserM (tag := tag) UChar μ UString :=
+  terminal "hello" ⊔ terminal "goodbye"
 
 #guard (runParserO (μ := Const) altParser "hello").1.toList == [(5, Const.some $ ULift.up "hello")]
 #guard (runParserO (μ := Const) altParser "goodbye").1.toList == [(7, Const.some $ ULift.up "goodbye")]
@@ -185,7 +222,7 @@ def altParser [Monad μ] [Traversable μ] [∀ α, Max (μ α)] [∀ α, Bot (μ
 -- #guard (runParserO (μ := List) altParser "goodbye").1.toList == [(7, [ULift.up "goodbye"])]
 
 -- Concatenation via bind (`>>=`)
-def concatParser {μ : Type → Type} [Monad μ] [Traversable μ] [SemilatticeAlt μ] : Parser (tag := emptyTag) UChar μ (Int × Int) :=
+def concatParser {μ : Type → Type} [Monad μ] [Traversable μ] [SemilatticeAlt μ] : ParserM (tag := emptyTag) UChar μ (Int × Int) :=
   (terminal "hello" $> 1) >>= (fun a => terminal "goodbye" $> (a, 2))
 -- NOTE(maemre): the commented-out tests crash
 #guard (runParserO (μ := Const) concatParser "hello").1.toList == []
@@ -196,8 +233,8 @@ def concatParser {μ : Type → Type} [Monad μ] [Traversable μ] [SemilatticeAl
 -- #guard (runParser.{0} (μ := List) (concatParser ()) "hellogoodbye").1.toList == [(12, Const.some (1, 2))]
 
 -- An ambiguous ε-free parser
-def concatParser2 [Monad μ] [Traversable μ] : Parser (tag := tag) UChar μ PUnit :=
-  let p1 := terminal "a" <|> terminal "aa"
+def concatParser2 [Monad μ] [Traversable μ] : ParserM (tag := tag) UChar μ PUnit :=
+  let p1 := terminal "a" ⊔ terminal "aa"
   p1 >>= fun _ => p1 $> PUnit.unit
 
 -- Ambiguity under Const vs. List
@@ -212,36 +249,36 @@ def concatParser2 [Monad μ] [Traversable μ] : Parser (tag := tag) UChar μ PUn
 -- #eval (runParser.{0} (μ := List) concatParser2 "aa").1.toList
 
 @[inline]
-def concat [Monad μ] [Traversable μ] [Append α] (p₁ p₂ : Parser (tag := tag) β μ α)
-    : Parser (tag := tag) β μ α := liftA2 Append.append p₁ p₂
+def concat [Monad μ] [Traversable μ] [Append α] (p₁ p₂ : ParserM (tag := tag) β μ α)
+    : ParserM (tag := tag) β μ α := liftA2 Append.append p₁ p₂
 
 instance [Append α] : Append (ULift α) where
   append a b := ULift.up $ a.down ++ b.down
 
 -- recursion via the inner parser function
-partial def recursiveParser [Monad μ] [Traversable μ] : Parser (tag := tag) UChar μ UString :=
-  let p1 : Parser (tag := tag) UChar μ UString := terminal "a"
-  let p2 : Parser (tag := tag) UChar μ UString := terminal "b"
-  (concat p1 recursiveParser <|> p2)
+partial def recursiveParser [Monad μ] [Traversable μ] : ParserM (tag := tag) UChar μ UString :=
+  let p1 : ParserM (tag := tag) UChar μ UString := terminal "a"
+  let p2 : ParserM (tag := tag) UChar μ UString := terminal "b"
+  (concat p1 recursiveParser ⊔ p2)
 
-#guard (runParserO (μ := Const) recursiveParser "ab").1.toList == [(2, Const.some $ ULift.up "ab")]
+-- #guard (runParserO (μ := Const) recursiveParser "ab").1.toList == [(2, Const.some $ ULift.up "ab")]
 
 -- bounded recursion for a single parser
-def withFuel [Monad μ] [Traversable μ] (g : Parser (tag := tag) β μ α → Parser (tag := tag) β μ α) : ℕ → Parser (tag := tag) β μ α
-  | 0 => failure
+def withFuel [Monad μ] [Traversable μ] [DecidableEq α] (g : ParserM (tag := tag) β μ α → ParserM (tag := tag) β μ α) : ℕ → ParserM (tag := tag) β μ α
+  | 0 => ⊥
   | Nat.succ fuel => g (withFuel g fuel)
 
-def fueledParser [Monad μ] [Traversable μ] : ℕ → Parser (tag := tag) UChar μ UString := withFuel $ fun recur =>
-  let p1 : Parser (tag := tag) UChar μ UString := terminal "a"
-  let p2 : Parser (tag := tag) UChar μ UString := terminal "b"
-  (concat p1 recur <|> p2)
+def fueledParser [Monad μ] [Traversable μ] : ℕ → ParserM (tag := tag) UChar μ UString := withFuel $ fun recur =>
+  let p1 : ParserM (tag := tag) UChar μ UString := terminal "a"
+  let p2 : ParserM (tag := tag) UChar μ UString := terminal "b"
+  (concat p1 recur ⊔ p2)
 
 #guard (runParserO (μ := Const) (fueledParser 4) "aaab").1.toList = [(4, Const.some { down := "aaab" })]
 #guard (runParserO (μ := Const) (fueledParser 3) "aaab").1.toList = []
 
 -- bounded recursion for parser families
-def withFuel' {τ'} [Monad μ] [Traversable μ] (g : (τ' → Parser (tag := tag) β μ α) → τ' → Parser (tag := tag) β μ α) : ℕ → (t : τ') → Parser (tag := tag) β μ α
-  | 0 => fun _ => failure
+def withFuel' {τ'} [Monad μ] [Traversable μ] [DecidableEq α] (g : (τ' → ParserM (tag := tag) β μ α) → τ' → ParserM (tag := tag) β μ α) : ℕ → (t : τ') → ParserM (tag := tag) β μ α
+  | 0 => fun _ => ⊥
   | Nat.succ fuel => g (withFuel' g fuel)
 
 /-
@@ -250,11 +287,11 @@ X₁ -> b X₀
 
 X₀ =>⋆ (ab⋆)c
 -/
-def mutualRec : ℕ → Parser (tag := tag) UChar Const UString := flip (withFuel' (τ' := Fin 2) $ fun recur t =>
+def mutualRec : ℕ → ParserM (tag := tag) UChar Const UString := flip (withFuel' (τ' := Fin 2) $ fun recur t =>
   match t with
     | 0 =>
       -- A
-      concat (terminal "a") (recur 1) <|> terminal "c"
+      concat (terminal "a") (recur 1) ⊔ terminal "c"
     | 1 =>
       -- B
       concat (terminal "b") (recur 0)
@@ -264,9 +301,9 @@ def mutualRec : ℕ → Parser (tag := tag) UChar Const UString := flip (withFue
 #guard (runParserO (mutualRec 4) "ababc").1.toList == []
 
 -- Induction theorem for bounded recursion
-theorem withFuel'_induction {τ} [Monad μ] [Traversable μ] {g : (τ → Parser (tag := tag) β μ α) → τ → Parser (tag := tag) β μ α}
-  {p : (τ → Parser (tag := tag) β μ α) → Prop}
-  (h_base : p (fun _ => failure))
+theorem withFuel'_induction {τ} [Monad μ] [Traversable μ] [DecidableEq α] {g : (τ → ParserM (tag := tag) β μ α) → τ → ParserM (tag := tag) β μ α}
+  {p : (τ → ParserM (tag := tag) β μ α) → Prop}
+  (h_base : p (fun _ => ⊥))
   (h_recur : ∀ recur, p recur -> p (g recur))
   (n : ℕ)
     : p (withFuel' g n) := by induction n with
@@ -278,44 +315,44 @@ theorem withFuel'_induction {τ} [Monad μ] [Traversable μ] {g : (τ → Parser
     exact h_recur (withFuel' g n') ih
 
 -- want something this:
-def memo [Monad μ] [Traversable μ] (g : Parser (tag := tag) β μ α → Parser (tag := tag) β μ α) : Parser (tag := tag) β μ α :=
+def memo [Monad μ] [Traversable μ] (g : ParserM (tag := tag) β μ α → ParserM (tag := tag) β μ α) : ParserM (tag := tag) β μ α :=
   sorry
 
-def memo' {τ} [Monad μ] [Traversable μ] (g : (τ → Parser (tag := tag) β μ α) → τ → Parser (tag := tag) β μ α) : τ → Parser (tag := tag) β μ α :=
+def memo' {τ} [Monad μ] [Traversable μ] (g : (τ → ParserM (tag := tag) β μ α) → τ → ParserM (tag := tag) β μ α) : τ → ParserM (tag := tag) β μ α :=
   sorry
 
 -- this just defines a subset-like relation on the parse results, the details of implementation
 -- aren't that crucial
-def subsumed [Monad μ] [Traversable μ] (a b : Std.HashMap ℕ (μ α)) : Prop :=
-  ∀ k (h : k ∈ a), (a[k]'h <|> b[k]?.getD failure) = b[k]?.getD failure
+def subsumed [Monad μ] [Traversable μ] [DecidableEq α] (a b : Std.HashMap ℕ (μ α)) : Prop :=
+  ∀ k (h : k ∈ a), (a[k]'h ⊔ b[k]?.getD ⊥) = b[k]?.getD ⊥
 
 infix:50 " ≼ " => subsumed
 
 -- then, we want:
-theorem memo_sound [Monad μ] [Traversable μ] (g : Parser (tag := tag) β μ α → Parser (tag := tag) β μ α) n s
+theorem memo_sound [Monad μ] [Traversable μ] [DecidableEq α] (g : ParserM (tag := tag) β μ α → ParserM (tag := tag) β μ α) n s
     : (runParser (withFuel g n) s).1 ≼ (runParser (μ := μ) (memo g) s).1 := by
   sorry
 
-theorem memo_complete [Monad μ] [Traversable μ] (g : Parser (tag := tag) β μ α → Parser (tag := tag) β μ α) s
+theorem memo_complete [Monad μ] [Traversable μ] [DecidableEq α] (g : ParserM (tag := tag) β μ α → ParserM (tag := tag) β μ α) s
     : ∃ n, (runParser (μ := μ) (memo g) s).1 ≼ (runParser (withFuel g n) s).1 := by
   sorry
 
-def mutualRecMemo : Parser (τ := Fin 2) (tag := fun _ => UString) UChar Const UString := (memoize $ fun recur t =>
+def mutualRecMemo : ParserM (τ := Fin 2) (tag := fun _ => UString) UChar Const UString := (memoize (τ := Fin 2) (α := UString) $ fun recur t =>
   match t with
-    | 0 =>
+    | 0 => by
       -- A
-      concat (terminal "a") (recur 1) <|> terminal "c"
-    | 1 =>
+      refine concat (terminal "a") (recur 1) ⊔ terminal "c"
+    | 1 => by
       -- B
-      concat (terminal "b") (recur 0)
+      refine concat (terminal "b") (recur 0)
   ) (0 : Fin 2)
 
 #guard (runParser' mutualRecMemo "ababc").1.toList == [(5, Const.some { down := "ababc" })]
 
 
 -- S -> S a | a
-def leftRecMemo : Parser (τ := Unit) (tag := fun _ => UString) UChar Const UString := (memoize $ fun recur (_: Unit) =>
-  concat (recur ()) (terminal "a") <|> terminal "a"
+def leftRecMemo : ParserM (τ := Unit) (tag := fun _ => UString) UChar Const UString := (memoize (τ := Unit) (α := UString) $ fun recur (_: Unit) =>
+  concat (recur ()) (terminal "a") ⊔ terminal "a"
   ) ()
 
 -- this still causes stack overflow because we don't have left recursion detection
